Fix StepStar definitions, generalize chasles_step_star theorem and add step_to_stepstar lemma

ExprEval/Arithmetic.lean
@@ -46,6 +46,6 @@ inductive ArStep: (val: V -> Int) -> (ArExpr V) -> (ArExpr V) -> Prop where
     | subRight (n: Int) (e₂ e₂': ArExpr V) : ArStep val e₂ e₂' -> ArStep val (ArExpr.Sub (ArExpr.Const n) e₂)  (ArExpr.Sub (ArExpr.Const n) e₂')
     | mulRight (n: Int) (e₂ e₂': ArExpr V) : ArStep val e₂ e₂' -> ArStep val (ArExpr.Mul (ArExpr.Const n) e₂)  (ArExpr.Mul (ArExpr.Const n) e₂')
 
-def ArStepStar (V: Type) := StepStar (StepKind := ArStep V) V
-def ArStepStar.refl {V: Type} (val: V -> Int) := StepStar.refl (StepKind := ArStep V) val
-def ArStepStar.trans {V: Type} {val: V -> Int} e₁ e₂ e₃ := StepStar.trans e₁ e₂ e₃ (StepKind := ArStep V) (val := val)
+def ArStepStar (V: Type) := StepStar (Step := ArStep V) V
+def ArStepStar.refl {V: Type} (val: V -> Int) := StepStar.refl (Step := ArStep V) val
+def ArStepStar.trans {V: Type} {val: V -> Int} e₁ e₂ e₃ := StepStar.trans e₁ e₂ e₃ (Step := ArStep V) (val := val)
