ExprEval/Expr.lean
@@ -20,6 +20,26 @@ inductive BoolExpr : Type
     | And : BoolExpr -> BoolExpr -> BoolExpr
     | Or : BoolExpr -> BoolExpr -> BoolExpr
 
-inductive StepStar {ExprType: Type} {StepKind: (V -> Int) -> ExprType -> ExprType -> Prop} : (val: V -> Int) -> ExprType -> ExprType -> Prop where
+def StepKind (V: Type) (ExprType: Type):= (V -> Int) -> ExprType -> ExprType -> Prop
+
+inductive StepStar {ExprType: Type} {Step: StepKind V ExprType} : (val: V -> Int) -> ExprType -> ExprType -> Prop where
         | refl val e : StepStar val e e
-        | trans e₁ e₂ e₃ : StepKind val e₁ e₂ -> StepStar val e₂ e₃ -> StepStar val e₁ e₃
+        | trans e₁ e₂ e₃ : Step val e₁ e₂ -> StepStar val e₂ e₃ -> StepStar val e₁ e₃
+
+theorem chasles_step_star {ExprKind: Type} {Step: StepKind V ExprKind} {e₁ e₂ e₃: ExprKind}:
+    StepStar (Step := Step) V val e₁ e₂  ->
+        StepStar (Step := Step) V val e₂ e₃ ->
+            StepStar (Step := Step) V val e₁ e₃ := by
+    intros h1 h2
+    induction h1 with
+    | refl e => exact h2
+    | trans a b c step _ ihn =>
+        have h3 := ihn h2
+        have h4 := StepStar.trans _ _ _ step h3
+        exact h4
+
+theorem step_to_stepstar {ExprKind: Type} {Step: StepKind V ExprKind} {e e': ExprKind}:
+    Step val e e' -> StepStar (Step := Step) V val e e' := by
+    intro h
+    have h': StepStar (Step := Step) V val e' e' := StepStar.refl val e'
+    apply StepStar.trans _ _ _ h h'
